Add comment for later (about cycling)

Sigma.v
@@ -2029,6 +2029,24 @@ Section Sigma.
     - admit.
   Admitted.
 
+  (* Axiom take: NUMBER -> SUBST -> VECTOR.
+
+  Definition right_cycle (i k: NUMBER) e: TERM :=
+    traverse (subst_app (take i (subst_lift 1) ++ [var 0]) (subst_lift (succ i))) k e.
+
+  Definition left_cycle (i k: NUMBER) e: TERM :=
+    subst (var i) k (lift 1 (1 + i + k) e).
+
+  Goal
+    forall i k e,
+    joinable (right_cycle i k (left_cycle i k e))
+             (left_cycle i k (right_cycle i k e)).
+  Proof.
+    unfold left_cycle.
+    unfold right_cycle.
+    intros.
+    why?. *)
+
   (* ---------------------------------------------------------------------- *)
 
   Hint Resolve clos_rt_rt1n: sigma.
